\documentclass[12pt, letterpaper]{article}
\begin{document}
\setlength\parindent{0pt}
Solve the ODE by integration or by remembering a differentiation formula: 
\[ y' = 4e^{-x}cosx \]
Solution:
This problem can be solved as an integration by parts. As a reminder, integration by parts
uses the differentiation product rule:
\[ \frac{d}{dx}[u*v] = \frac{du}{dx}v + u\frac{dv}{dx} \]
Which can be manipulated using the fundamental theorem of calculus:
\[ uv = \int{\frac{du}{dx}v}\,dx + \int{u\frac{dv}{dx}}\,dx \]
Or as it is often written:
\[ \int{u'v}\,dx = uv - \int{uv'}\,dx \] 
The idea generally being that we can "reduce" the complexity of the equation by 
differentiating and integrating the terms separately. This particular problem is a 
variation of a canonical problem in integral calculus and requires an algebraic trick 
to solve.
In this case, we will set $y' = u'v$ where $4e^{-x} = u'$ and $cosx = v$. Thus:
\[ \int{y'}\,dx = y = uv - \int{uv'}\,dx \]
We know $u'$, $v$, and must find $u$ and $v'$ by integration and differentiation, 
respectively. $u$ will be:
\[ \int{4e^{-x}}\,dx = -4e^{-x} \]
And then, $v'$ is:
\[ \frac{dcosx}{dx} = -sinx \]
Then we can write:
\[ y = -4e^{-x}cosx - \int{-4e^{-x}*-sinx}\,dx \]
Cleaning up a bit:
\[ y = -4e^{-x}cosx - \int{4e^{-x}sinx}\,dx \]
Next, we will perform a second round of integration by parts on the term: 
\[ \int{4e^{-x}sinx}\,dx \]
Where, similar to before, $u' = 4e^{-x}$ and $v = sinx$. And we must solve for $u$ and $v'$:
\[ u = \int{4e^{-x}}\,dx = -4e^{-x} \]
And:
\[ v' = \frac{dsinx}{dx} = cosx \]
Then:
\[ \int{4e^{-x}sinx}\,dx = -4e^{-x}sinx - \int{-4e^{-x}cosx}\,dx \]
From here, we go back to our earlier equation:
\[ y = -4e^{-x}cosx - \int{4e^{-x}sinx}\,dx \]
And we will substitute $-4e^{-x}sinx - \int{-4e^{-x}cosx}\,dx$ for $\int{4e^{-x}sinx}\,dx$:
\[ y = -4e^{-x}cosx - (-4e^{-x}sinx - \int{-4e^{-x}cosx}\,dx) \]
Cleaning up a bit:
\[ y = -4e^{-x}cosx + 4e^{-x}sinx - \int{4e^{-x}cosx}\,dx \]
Recall from the very beginning 
\[ y' = 4e^{-x}cosx \]
And therefore:
\[ y = \int{4e^{-x}cosx}\,dx\]
Notice that $y$ appears on both sides of the equation:
\[ y = -4e^{-x}cosx + 4e^{-x}sinx - y \]
And then we can rearrange:
\[ 2y = -4e^{-x}cosx + 4e^{-x}sinx \]
Finally:
\[ y = \frac{-4e^{-x}cosx + 4e^{-x}sinx}{2} + C\]
\end{document}